theories/models/utp_vdm_simple/utp_vdm_sorts.thy
@@ -1,139 +1,145 @@
 theory utp_vdm_sorts
 imports 
   "../../core/utp_sorts"
-  "../../alpha/utp_alpha_pred" 
-  "../../alpha/utp_alpha_map" 
   utp_vdm_inject 
 begin
 
-instantiation vdmval :: VALUE
+instantiation vdmv :: VALUE
 begin
 
 (*
 definition utype_rel_vval :: "vval \<Rightarrow> nat \<Rightarrow> bool" where
-"utype_rel_vval x u = \<exists> t :: vdmtype. u = emb\<cdot>(Def t) \<and> x :\<^sub>v t)"
+"utype_rel_vval x u = \<exists> t :: vdmt. u = emb\<cdot>(Def t) \<and> x :\<^sub>v t)"
 *)
 
 lemma Defined_nbot [simp]: "\<D>\<^sub>v x \<Longrightarrow> x \<noteq> BotV"
   by (auto)
 
-definition utype_rel_vdmval :: "vdmval \<Rightarrow> nat \<Rightarrow> bool" where
-"utype_rel_vdmval x u = (\<exists> t :: vdmtype. u = to_nat t \<and> x :\<^sub>v t)"
+definition utype_rel_vdmv :: "vdmv \<Rightarrow> nat \<Rightarrow> bool" where
+"utype_rel_vdmv x u = (\<exists> t :: vdmt. u = to_nat t \<and> x :\<^sub>v t)"
 
-definition Defined_vdmval :: "vdmval \<Rightarrow> bool" where
-"Defined_vdmval \<equiv> \<D>\<^sub>v"
+definition Defined_vdmv :: "vdmv \<Rightarrow> bool" where
+"Defined_vdmv \<equiv> \<D>\<^sub>v"
 
 instance
   apply (intro_classes)
-  apply (simp add:utype_rel_vdmval_def Defined_vdmval_def)
+  apply (simp add:utype_rel_vdmv_def Defined_vdmv_def)
   apply (rule_tac x="to_nat BoolT" in exI)
   apply (force)
 done
 end
 
-lemma vdmtype_UTYPE [simp]: "\<lbrakk> v :\<^sub>v t; \<D> v \<rbrakk> \<Longrightarrow> to_nat t \<in> UTYPES (TYPE(vdmval))"
-  by (auto simp add:UTYPES_def utype_rel_vdmval_def)
+lemma vdmt_UTYPE [simp]: "\<lbrakk> v :\<^sub>v t; \<D> v \<rbrakk> \<Longrightarrow> to_nat t \<in> UTYPES (TYPE(vdmv))"
+  by (auto simp add:UTYPES_def utype_rel_vdmv_def)
 
 lemma prjTYPE_inv_vdm [simp]
-  : "embTYPE ((prjTYPE t) :: vdmtype) = (t :: vdmval UTYPE)"
+  : "embTYPE ((prjTYPE t) :: vdmt) = (t :: vdmv UTYPE)"
   apply (simp add:prjTYPE_def embTYPE_def)
   apply (case_tac t)
-  apply (auto simp add: utype_rel_vdmval_def UTYPES_def)
+  apply (auto simp add: utype_rel_vdmv_def UTYPES_def)
 done
 
-lemma type_rel_vdmtype_exists: 
-  "(x::vdmval) : a \<Longrightarrow> \<exists> t. a = embTYPE t \<and> x :\<^sub>v t" 
+lemma embTYPE_inv_vbtypes [simp]:
+  "t \<in> vbtypes \<Longrightarrow> prjTYPE (embTYPE t :: vdmv UTYPE) = t"
+  apply (auto simp add:vbtypes_def)
+  apply (rule_tac v="BasicV x" in embTYPE_inv)
+  apply (auto simp add: utype_rel_vdmv_def Defined_vdmv_def)
+done
+
+lemma type_rel_vdmt_exists: 
+  "(x::vdmv) : a \<Longrightarrow> \<exists> t. a = embTYPE t \<and> x :\<^sub>v t" 
   apply (simp add:type_rel_def)
-  apply (simp add:utype_rel_vdmval_def)
+  apply (simp add:utype_rel_vdmv_def)
   apply (case_tac a)
   apply (auto simp add:UTYPES_def)
   apply (rule_tac x="t" in exI)
   apply (simp add:embTYPE_def)
 done
 
-lemma type_rel_vdmtype_elim [elim]:
-  "\<lbrakk>(x::vdmval) : a; \<And> t. \<lbrakk> a = embTYPE t; x :\<^sub>v t \<rbrakk> \<Longrightarrow> P \<rbrakk> \<Longrightarrow> P"
-  by (metis type_rel_vdmtype_exists)
+lemma type_rel_vdmt_elim [elim]:
+  "\<lbrakk>(x::vdmv) : a; \<And> t. \<lbrakk> a = embTYPE t; x :\<^sub>v t \<rbrakk> \<Longrightarrow> P \<rbrakk> \<Longrightarrow> P"
+  by (metis type_rel_vdmt_exists)
 
 lemma BotV_type: "BotV :\<^sub>v a"
   by (auto)
 
-lemma type_rel_vdmtype [simp]: "x : t \<longleftrightarrow> x :\<^sub>v prjTYPE t"
-  apply (auto simp add: type_rel_def utype_rel_vdmval_def prjTYPE_def)
-  apply (metis Rep_UTYPE_elim from_nat_to_nat utype_rel_vdmval_def)
+lemma type_rel_vdmt: 
+  "x : t \<longleftrightarrow> x :\<^sub>v prjTYPE t"
+  apply (auto simp add: type_rel_def utype_rel_vdmv_def prjTYPE_def)
+  apply (metis Rep_UTYPE_elim from_nat_to_nat utype_rel_vdmv_def)
 done
 
-instantiation vdmval :: BOT_SORT
+instantiation vdmv :: BOT_SORT
 begin
 
-definition ubot_vdmval :: "vdmval" where
-"ubot_vdmval = BotV"
+definition ubot_vdmv :: "vdmv" where
+"ubot_vdmv = BotV"
 
 instance
   apply (intro_classes)
-  apply (simp add:ubot_vdmval_def Defined_vdmval_def)
+  apply (simp add:ubot_vdmv_def Defined_vdmv_def)
 done
 end
 
-lemma Defined_bot [simp]: "\<D> (BotV :: vdmval) \<longleftrightarrow> False"
-  by (simp add:Defined_vdmval_def)
+lemma Defined_bot [simp]: "\<D> (BotV :: vdmv) \<longleftrightarrow> False"
+  by (simp add:Defined_vdmv_def)
 
 lemma Defined_ubot [simp]: "\<D> \<bottom>v \<longleftrightarrow> False"
-  by (simp add:Defined_vdmval_def)
+  by (simp add:Defined_vdmv_def)
 
 (*
-lemma vdmval_UTYPE_nbot [simp]: 
-  "(from_nat (Rep_UTYPE (t :: vdmval UTYPE)) :: vdmtype lift) \<noteq> \<bottom>"
+lemma vdmv_UTYPE_nbot [simp]: 
+  "(from_nat (Rep_UTYPE (t :: vdmv UTYPE)) :: vdmt lift) \<noteq> \<bottom>"
   apply (case_tac t)
-  apply (auto simp add: UTYPES_def utype_rel_vdmval_def)
+  apply (auto simp add: UTYPES_def utype_rel_vdmv_def)
   apply (auto)
 done
 
-lemma vdmval_UTYPE_Def [simp]: 
-  "\<exists> x. (prj\<cdot>(Rep_UTYPE (a :: vdmval UTYPE)) :: vdmtype lift) = Def x"
+lemma vdmv_UTYPE_Def [simp]: 
+  "\<exists> x. (prj\<cdot>(Rep_UTYPE (a :: vdmv UTYPE)) :: vdmt lift) = Def x"
   apply (case_tac a)
   apply (simp add: UTYPES_def)
-  apply (simp add: utype_rel_vdmval_def)
+  apply (simp add: utype_rel_vdmv_def)
   apply (auto)
 done
 
-lemma vdmval_UTYPE_elim [elim]:
-  assumes "\<And> x. (prj\<cdot>(Rep_UTYPE (a :: vdmval UTYPE)) :: vdmtype lift) = Def x \<Longrightarrow> P" 
+lemma vdmv_UTYPE_elim [elim]:
+  assumes "\<And> x. (prj\<cdot>(Rep_UTYPE (a :: vdmv UTYPE)) :: vdmt lift) = Def x \<Longrightarrow> P" 
   shows "P"
-  by (metis assms vdmval_UTYPE_Def)
+  by (metis assms vdmv_UTYPE_Def)
 *)
 subsection {* Int sort instantiation *}
 
-instantiation vdmval :: INT_SORT
+instantiation vdmv :: INT_SORT
 begin
 
-definition MkInt_vdmval where "MkInt_vdmval (x::int) = InjVB x"
-definition DestInt_vdmval where "DestInt_vdmval x = (ProjVB x :: int)"
-definition IntUType_vdmval :: "vdmval itself \<Rightarrow> nat" where 
-"IntUType_vdmval = (\<lambda> x. to_nat IntT)"
+definition MkInt_vdmv where "MkInt_vdmv (x::int) = InjVB x"
+definition DestInt_vdmv where "DestInt_vdmv x = (ProjVB x :: int)"
+definition IntUType_vdmv :: "vdmv itself \<Rightarrow> nat" where 
+"IntUType_vdmv = (\<lambda> x. to_nat IntT)"
 
 instance 
-  apply (intro_classes, simp_all add:MkInt_vdmval_def DestInt_vdmval_def IntUType_vdmval_def type_rel_def utype_rel_vdmval_def embTYPE_def)
+  apply (intro_classes, simp_all add:MkInt_vdmv_def DestInt_vdmv_def IntUType_vdmv_def type_rel_def utype_rel_vdmv_def embTYPE_def)
   apply (auto)
-  apply (simp_all add: Inject_int_def InjVB_def Defined_vdmval_def MkInt_vdmval_def image_def)
+  apply (simp_all add: Inject_int_def InjVB_def Defined_vdmv_def MkInt_vdmv_def image_def)
   apply (force)+
 done
 end
 
 subsection {* Bool sort instantiation *}
 
-instantiation vdmval :: BOOL_SORT
+instantiation vdmv :: BOOL_SORT
 begin
 
-definition MkBool_vdmval where "MkBool_vdmval (x::bool) = InjVB x"
-definition DestBool_vdmval where "DestBool_vdmval x = (ProjVB x :: bool)"
-definition BoolUType_vdmval :: "vdmval itself \<Rightarrow> nat" where 
-"BoolUType_vdmval = (\<lambda>x. to_nat BoolT)"
+definition MkBool_vdmv where "MkBool_vdmv (x::bool) = InjVB x"
+definition DestBool_vdmv where "DestBool_vdmv x = (ProjVB x :: bool)"
+definition BoolUType_vdmv :: "vdmv itself \<Rightarrow> nat" where 
+"BoolUType_vdmv = (\<lambda>x. to_nat BoolT)"
 
 instance 
-  apply (intro_classes, simp_all add:MkBool_vdmval_def DestBool_vdmval_def BoolUType_vdmval_def type_rel_def utype_rel_vdmval_def embTYPE_def)
+  apply (intro_classes, simp_all add:MkBool_vdmv_def DestBool_vdmv_def BoolUType_vdmv_def type_rel_def utype_rel_vdmv_def embTYPE_def)
   apply (auto)
-  apply (simp_all add:InjVB_def Inject_bool_def Defined_vdmval_def MkBool_vdmval_def image_def)
+  apply (simp_all add:InjVB_def Inject_bool_def Defined_vdmv_def MkBool_vdmv_def image_def)
   apply (force)
   apply (erule vbtypes_type_cases)
   apply (auto)
@@ -142,49 +148,49 @@ end
 
 subsection {* Set sort instantiation *}
 
-instantiation vdmval :: SET_SORT_PRE
+instantiation vdmv :: SET_SORT_PRE
 begin
 
-  definition MkSet_vdmval :: "vdmval set \<Rightarrow> vdmval" where
-  "MkSet_vdmval xs = SetV (ProjBasicV ` xs)"
+  definition MkSet_vdmv :: "vdmv set \<Rightarrow> vdmv" where
+  "MkSet_vdmv xs = SetV (ProjBasicV ` xs)"
   
-  definition DestSet_vdmval :: "vdmval \<Rightarrow> vdmval set" where
-  "DestSet_vdmval v = BasicV ` ProjSetV v"
+  definition DestSet_vdmv :: "vdmv \<Rightarrow> vdmv set" where
+  "DestSet_vdmv v = BasicV ` ProjSetV v"
 
-  definition IsSetElemType_vdmval :: "vdmval UTYPE \<Rightarrow> bool" where
-  "IsSetElemType_vdmval t = (prjTYPE t \<in> vbtypes)"
+  definition IsSetElemType_vdmv :: "vdmv UTYPE \<Rightarrow> bool" where
+  "IsSetElemType_vdmv t = (prjTYPE t \<in> vbtypes)"
 
-  definition SetType_vdmval :: "vdmval UTYPE \<Rightarrow> vdmval UTYPE" where
-  "SetType_vdmval t = embTYPE (SetT (prjTYPE t))"
+  definition SetType_vdmv :: "vdmv UTYPE \<Rightarrow> vdmv UTYPE" where
+  "SetType_vdmv t = embTYPE (SetT (prjTYPE t))"
 
 instance ..
 
 end
 
 lemma embTYPE_inv_SetT:
-  "prjTYPE (embTYPE (SetT t) :: vdmval UTYPE) = SetT t"
+  "prjTYPE (embTYPE (SetT t) :: vdmv UTYPE) = SetT t"
   apply (rule_tac embTYPE_inv[of "SetV {}"])
-  apply (auto simp add: utype_rel_vdmval_def Defined_vdmval_def)
+  apply (auto simp add: utype_rel_vdmv_def Defined_vdmv_def)
 done
 
-instantiation vdmval :: SET_SORT
+instantiation vdmv :: SET_SORT
 begin
 
 instance
   apply (intro_classes)
-  apply (auto simp add:DestSet_vdmval_def MkSet_vdmval_def SetType_vdmval_def IsSetElemType_vdmval_def)
+  apply (auto simp add:DestSet_vdmv_def MkSet_vdmv_def SetType_vdmv_def IsSetElemType_vdmv_def type_rel_vdmt)
   apply (drule_tac x="xb" in bspec)
   apply (simp)
   apply (force)
   apply (force)
-  apply (simp_all add:dcarrier_def)
+  apply (simp_all add:dcarrier_def type_rel_vdmt)
   apply (auto)
-  apply (subgoal_tac "\<exists> v::vdmval. v :\<^sub>u to_nat (SetT (prjTYPE t)) \<and> \<D> v")
+  apply (subgoal_tac "\<exists> v::vdmv. v :\<^sub>u to_nat (SetT (prjTYPE t)) \<and> \<D> v")
   apply (force)
   apply (rule_tac x="SetV {}" in exI)
-  apply (auto simp add:utype_rel_vdmval_def Defined_vdmval_def embTYPE_inv_SetT)
+  apply (auto simp add:utype_rel_vdmv_def Defined_vdmv_def embTYPE_inv_SetT)
   apply (metis (lifting) CollectD IsBasicV.simps(1) ProjBasicV_inv set_mp vbtypes_type_cases vdefined.simps(1))
-  apply (simp add:image_def MkSet_vdmval_def)
+  apply (simp add:image_def MkSet_vdmv_def)
   apply (erule SetT_type_cases)
   apply (auto)
   apply (rule_tac x="BasicV ` xs" in bexI)
@@ -201,31 +207,31 @@ lemma ProjBasicV_not_basic [simp]: "\<not> IsBasicV x \<Longrightarrow> ProjBasi
   by (case_tac x, auto)
 
 lemma embTYPE_inv_FuncT:
-  "prjTYPE (embTYPE (a → b) :: vdmval UTYPE) = (a → b)"
+  "prjTYPE (embTYPE (a → b) :: vdmv UTYPE) = (a → b)"
   apply (rule_tac embTYPE_inv[of "FuncV (\<lambda> x. BotV)"])
-  apply (auto simp add: utype_rel_vdmval_def Defined_vdmval_def)
+  apply (auto simp add: utype_rel_vdmv_def Defined_vdmv_def)
 done
 
-instantiation vdmval :: FUNCTION_SORT
+instantiation vdmv :: FUNCTION_SORT
 begin
 
-definition "MkFunc_vdmval f = FuncV (f \<circ> BasicV)"
-definition "DestFunc_vdmval f = (\<lambda> x. (ProjFuncV f) (ProjBasicV x))"
-definition "IsFunc_vdmval f = ({x. f x \<noteq> BotV} \<subseteq> range BasicV \<and> f BotV = BotV)"
-definition FuncType_vdmval :: "vdmval UTYPE \<Rightarrow> vdmval UTYPE \<Rightarrow> vdmval UTYPE" where
-"FuncType_vdmval a b = embTYPE (FuncT (prjTYPE a) (prjTYPE b))"
+definition "MkFunc_vdmv f = FuncV (f \<circ> BasicV)"
+definition "DestFunc_vdmv f = (\<lambda> x. (ProjFuncV f) (ProjBasicV x))"
+definition "IsFunc_vdmv f = ({x. f x \<noteq> BotV} \<subseteq> range BasicV \<and> f BotV = BotV)"
+definition FuncType_vdmv :: "vdmv UTYPE \<Rightarrow> vdmv UTYPE \<Rightarrow> vdmv UTYPE" where
+"FuncType_vdmv a b = embTYPE (FuncT (prjTYPE a) (prjTYPE b))"
 
 instance 
   apply (intro_classes)
   apply (rule ext)
-  apply (simp add:DestFunc_vdmval_def MkFunc_vdmval_def IsFunc_vdmval_def FuncType_vdmval_def)
+  apply (simp add:DestFunc_vdmv_def MkFunc_vdmv_def IsFunc_vdmv_def FuncType_vdmv_def type_rel_vdmt)
   apply (clarify)
   apply (case_tac "IsBasicV x")
   apply (simp)
   apply (simp add: subset_iff)
   apply (metis IsBasicV.simps(1) image_iff)
-  apply (metis Defined_vdmval_def MkFunc_vdmval_def vdefined.simps(3))
-  apply (simp add:MkFunc_vdmval_def IsFunc_vdmval_def dcarrier_def FuncType_vdmval_def embTYPE_inv_FuncT Defined_vdmval_def)
+  apply (metis Defined_vdmv_def MkFunc_vdmv_def vdefined.simps(3))
+  apply (simp add:MkFunc_vdmv_def IsFunc_vdmv_def dcarrier_def FuncType_vdmv_def embTYPE_inv_FuncT Defined_vdmv_def type_rel_vdmt)
   apply (auto)
   apply (rule)
   apply (force)
@@ -243,54 +249,54 @@ instance
   apply (simp)
   apply (smt ProjBasicV_not_basic UNIV_I image_iff mem_Collect_eq subsetI utp_vdm_values.ProjBasicV_inv)
   apply (force)
-  apply (simp_all add:FuncType_vdmval_def)
-  apply (metis (lifting) embTYPE_inv_FuncT prjTYPE_inv_vdm vdmtype.simps(9))+
+  apply (simp_all add:FuncType_vdmv_def)
+  apply (metis (lifting) embTYPE_inv_FuncT prjTYPE_inv_vdm vdmt.simps(9))+
 done
 
 end
 
 
 (*
-instantiation vdmval :: FUNCTION_SORT
+instantiation vdmv :: FUNCTION_SORT
 begin
 
-definition MkFunc_vdmval where "MkFunc_vdmval f = FuncV\<cdot>(\<Lambda>! x. f x)"
-definition DestFunc_vdmval where "DestFunc_vdmval f \<equiv> \<lambda> x. (sfun_rep\<cdot>(ProjFuncV\<cdot>f))\<cdot>x"
-definition IsFunc_vdmval :: "(vdmval \<Rightarrow> vdmval) \<Rightarrow> bool" where
-"IsFunc_vdmval f \<equiv> cont f \<and> f \<bottom> = \<bottom> \<and> (\<exists>x. x \<noteq> \<bottom> \<and> f x \<noteq> \<bottom>)"
-definition FuncType_vdmval :: "vdmval UTYPE \<Rightarrow> vdmval UTYPE \<Rightarrow> vdmval UTYPE" where
-"FuncType_vdmval a b \<equiv>
+definition MkFunc_vdmv where "MkFunc_vdmv f = FuncV\<cdot>(\<Lambda>! x. f x)"
+definition DestFunc_vdmv where "DestFunc_vdmv f \<equiv> \<lambda> x. (sfun_rep\<cdot>(ProjFuncV\<cdot>f))\<cdot>x"
+definition IsFunc_vdmv :: "(vdmv \<Rightarrow> vdmv) \<Rightarrow> bool" where
+"IsFunc_vdmv f \<equiv> cont f \<and> f \<bottom> = \<bottom> \<and> (\<exists>x. x \<noteq> \<bottom> \<and> f x \<noteq> \<bottom>)"
+definition FuncType_vdmv :: "vdmv UTYPE \<Rightarrow> vdmv UTYPE \<Rightarrow> vdmv UTYPE" where
+"FuncType_vdmv a b \<equiv>
   case (prj\<cdot>(Rep_UTYPE a), prj\<cdot>(Rep_UTYPE b)) of
     (Def a', Def b') \<Rightarrow> embTYPE (FuncT a' b') |
-    _ \<Rightarrow> Abs_UTYPE (emb\<cdot>(\<bottom> :: vdmtype lift))"
+    _ \<Rightarrow> Abs_UTYPE (emb\<cdot>(\<bottom> :: vdmt lift))"
 
 instance proof
-  fix f :: "vdmval \<Rightarrow> vdmval"
+  fix f :: "vdmv \<Rightarrow> vdmv"
 
   assume isFunc: "IsFunc f"
   from isFunc show "DestFunc (MkFunc f) = f"
-    by (simp add:MkFunc_vdmval_def DestFunc_vdmval_def IsFunc_vdmval_def)
+    by (simp add:MkFunc_vdmv_def DestFunc_vdmv_def IsFunc_vdmv_def)
 
   from isFunc show "\<D> (MkFunc f)"
-    apply (auto simp add:Defined_vdmval_def IsFunc_vdmval_def MkFunc_vdmval_def FuncType_vdmval_def sfun_eq_iff)
+    apply (auto simp add:Defined_vdmv_def IsFunc_vdmv_def MkFunc_vdmv_def FuncType_vdmv_def sfun_eq_iff)
     apply (metis Abs_cfun_inverse2 Rep_cfun_strict1)
   done
 
-  fix a b :: "vdmval UTYPE"
+  fix a b :: "vdmv UTYPE"
   assume funcRange: "\<forall>x. x : a \<longrightarrow> f x : b"
   from isFunc funcRange show "MkFunc f : FuncType a b"
-    apply (auto simp add: MkFunc_vdmval_def type_rel_def utype_rel_vdmval_def IsFunc_vdmval_def)
-    apply (simp add:FuncType_vdmval_def)
-    apply (insert vdmval_UTYPE_Def[of "a"])
+    apply (auto simp add: MkFunc_vdmv_def type_rel_def utype_rel_vdmv_def IsFunc_vdmv_def)
+    apply (simp add:FuncType_vdmv_def)
+    apply (insert vdmv_UTYPE_Def[of "a"])
     apply (erule exE)
     apply (simp)
-    apply (insert vdmval_UTYPE_Def[of "b"])
+    apply (insert vdmv_UTYPE_Def[of "b"])
     apply (erule exE)
     apply (simp add:embTYPE_def)
 
     apply (rule FuncV_type)
     apply (auto)
-    apply (metis (lifting) BasicV_type Rep_UTYPE_elim emb_inverse lift.inject utype_rel_vdmval_def)
+    apply (metis (lifting) BasicV_type Rep_UTYPE_elim emb_inverse lift.inject utype_rel_vdmv_def)
   done
 qed
 end
@@ -298,178 +304,28 @@ end
 lemma carrier_vcarrier [simp]: "carrier t = vcarrier (prjTYPE t)"
   by (simp add:carrier_def vcarrier_def)
 
-lemma prjTYPE_vdmval_IntT [simp]: 
-  "prjTYPE (IntType :: vdmval UTYPE) = IntT"
-  by (auto intro!: embTYPE_inv simp add:utype_rel_vdmval_def IntType_vdmval_def)
+lemma prjTYPE_vdmv_IntT [simp]: 
+  "prjTYPE (IntType :: vdmv UTYPE) = IntT"
+  by (auto intro!: embTYPE_inv simp add:utype_rel_vdmv_def IntType_vdmv_def)
 
-lemma prjTYPE_vdmval_BoolT [simp]: 
-  "prjTYPE (BoolType :: vdmval UTYPE) = BoolT"
-  by (auto intro!: embTYPE_inv simp add:utype_rel_vdmval_def BoolType_vdmval_def)
+lemma prjTYPE_vdmv_BoolT [simp]: 
+  "prjTYPE (BoolType :: vdmv UTYPE) = BoolT"
+  by (auto intro!: embTYPE_inv simp add:utype_rel_vdmv_def BoolType_vdmv_def)
 
-lemma prjTYPE_vdmval_FuncT [simp]:
-  "prjTYPE (FuncType a b :: vdmval UTYPE) = prjTYPE a → prjTYPE b"
+lemma prjTYPE_vdmv_FuncT [simp]:
+  "prjTYPE (FuncType a b :: vdmv UTYPE) = prjTYPE a → prjTYPE b"
   apply (case_tac a)
   apply (simp)
-  apply (simp add:FuncType_vdmval_def)
-  apply (insert vdmval_UTYPE_Def[of a])
-  apply (insert vdmval_UTYPE_Def[of b])
+  apply (simp add:FuncType_vdmv_def)
+  apply (insert vdmv_UTYPE_Def[of a])
+  apply (insert vdmv_UTYPE_Def[of b])
   apply (erule exE)
   apply (erule exE)
   apply (simp)
   apply (auto)
-  apply (metis Abs_UTYPE_inverse Undef.simps embTYPE_def emb_inverse prjTYPE_def vdmtype_UTYPE)
+  apply (metis Abs_UTYPE_inverse Undef.simps embTYPE_def emb_inverse prjTYPE_def vdmt_UTYPE)
 done
 *)
 
-definition vdm_enc_var ::
-  "vdmval VAR \<Rightarrow> vbasic" where
-"vdm_enc_var v = RecI [NameI (name v), TypeI (prjTYPE (vtype v)), BoolI (aux v)]"
-
-definition vdm_dec_var ::
-  "vbasic \<Rightarrow> vdmval VAR" where
-"vdm_dec_var v = 
-  (let r = the (ProjRecI v) 
-    in MkVar (the (ProjNameI (r!0))) (embTYPE (the (ProjTypeI (r!1)))) (the (ProjBoolI (r!2))))"
-
-lemma vdm_enc_var_inv [simp]:
-  "vdm_dec_var (vdm_enc_var v) = v"
-  by (simp add:vdm_enc_var_def vdm_dec_var_def MkVar_def)
-
-abbreviation "VarT \<equiv> RecordT [NameT, TypeT, BoolT]"
-
-lemma vdm_enc_var_type [typing]:
-  "vdm_enc_var v :\<^sub>b VarT"
-  by (force simp add:vdm_enc_var_def)
-
-(*
-lemma "xs < ys \<Longrightarrow> RecI xs < RecI ys"
-*)
-
-lemma vdm_enc_var_strict_mono [simp]:
-  "strict_mono vdm_enc_var"
-  apply (simp add:strict_mono_def vdm_enc_var_def)
-  sorry
-
-definition vdm_enc_value :: "vdmval \<Rightarrow> vbasic" where
-"vdm_enc_value v = ProjBasicV v"
-
-fun vdm_dec_value :: "vbasic \<Rightarrow> vdmval" where
-"vdm_dec_value (OptionI (Some v)) = BasicV v" |
-"vdm_dec_value (OptionI None) = BotV" |
-"vdm_dec_value _ = BotV"
-
-lemma vdm_enc_value_inv [simp]:
-  "v \<in> vbvalues \<Longrightarrow> vdm_dec_value (vdm_enc_value v) = v"
-  apply (simp add:vdm_enc_value_def)
-  apply (case_tac v)
-  apply (simp_all add:vbvalues_def)
-done
-
-definition vdm_enc_binding :: 
-  "vdmval ALPHABET \<Rightarrow> vdmval WF_BINDING \<Rightarrow> vbasic" where
-"vdm_enc_binding a b =
-  (let bf = fmap_list (binding_fmap a b)
-    in PairI (FinI (map (vdm_enc_var \<circ> fst) bf)) (RecI (map (vdm_enc_value \<circ> snd) bf)))"
-
-fun vdm_dec_binding ::
-  "vbasic \<Rightarrow> vdmval WF_BINDING" where
-"vdm_dec_binding (PairI (FinI vs) (RecI bs)) 
-  = fmap_binding 
-      (list_fmap 
-         (zip (map vdm_dec_var vs) (map vdm_dec_value bs)))"
-
-lemma vdm_enc_binding_inv [simp]:
-  assumes "\<forall>v\<in>\<^sub>fa. prjTYPE (vtype v) \<in> vbtypes" 
-  shows "vdm_dec_binding (vdm_enc_binding a b) \<cong> b on \<langle>a\<rangle>\<^sub>f"
-proof -
-
-  have map_simp:
-        "map (vdm_dec_value \<circ> (vdm_enc_value \<circ> snd)) (fmap_list (binding_fmap a b)) =
-        map snd (fmap_list (binding_fmap a b))" (is "?A = ?B")
-  proof -
-    have "?A = map (vdm_dec_value \<circ> vdm_enc_value) (map snd (fmap_list (binding_fmap a b)))"
-      by (metis map_map)
-
-    also have "... = map snd (fmap_list (binding_fmap a b))"
-    proof -
-      from assms have "\<forall> x \<in> set (map snd (fmap_list (binding_fmap a b))). x \<in> vbvalues"
-        apply (simp add: fmap_list_binding_fmap)
-        apply (rule ballI)
-        apply (drule_tac x="x" in spec)
-        apply (simp)
-        apply (subgoal_tac "\<langle>b\<rangle>\<^sub>b x : vtype x")
-        apply (simp)
-        apply (erule vbtypes_type_cases)
-        apply (simp add:vbvalues_def)
-        apply (simp add:vbvalues_def)
-        apply (simp_all add:vbvalues_def vbtypes_def)
-        apply (force)
-        apply (metis binding_type type_rel_vdmtype)
-      done
-
-      with assms show ?thesis
-        by (metis (no_types) map_idI o_def vdm_enc_value_inv)
-    qed
-    
-    ultimately show ?thesis by simp
-
-  qed
-  
-  show ?thesis
-    apply (simp add:vdm_enc_binding_def)
-    apply (simp add:Let_def)
-    apply (simp add:map_simp)
-    apply (unfold comp_def)
-    apply (simp only: vdm_enc_var_inv zip_map_fst_snd)
-    apply (simp)
-    apply (subgoal_tac "vdm_dec_var \<circ> (vdm_enc_var \<circ> fst) = fst")
-    apply (metis binding_fmap_inv)
-    apply (simp add:comp_def)
-  done
-qed
-
-lemma vdm_enc_binding_type [typing]:
-  assumes "\<forall>v\<in>\<^sub>fa. prjTYPE (vtype v) \<in> vbtypes" 
-  shows "vdm_enc_binding a b :\<^sub>b  
-         PairT (FSetT VarT) (RecordT (map (OptionT \<circ> prjTYPE \<circ> vtype) (flist a)))"
-  proof -
-
-    obtain xs where xs_def: "a = fset xs" and xs_props: "distinct xs" "sorted xs"
-      by (metis flist_inv flist_props(1) flist_props(2))
-      
-    with assms have "\<forall>v\<in>\<^sub>ffset xs. prjTYPE (vtype v) \<in> vbtypes" 
-      by simp
-
-    with xs_props
-    have "map (\<lambda>x. vdm_enc_value (\<langle>b\<rangle>\<^sub>b x)) xs :\<^sub>r map (\<lambda>x. OptionT (prjTYPE (vtype x))) xs"
-    proof (induct xs)
-      case Nil thus ?case by (force)
-
-    next
-
-      case (Cons y ys)
-      thus ?case
-        apply (simp add:vdm_enc_value_def)
-        apply (rule)
-        apply (case_tac "\<langle>b\<rangle>\<^sub>b y = BotV")
-        apply (simp)
-        apply (force)
-
-        sorry
-    qed
-
-    with xs_props show ?thesis
-      apply (simp add:vdm_enc_binding_def Let_def)
-      apply (rule)
-      apply (rule)
-      apply (simp add: fmap_list_binding_fmap typing)
-      apply (simp add: map_map[THEN sym])
-      apply (metis flist_fimage flist_props(1) vdm_enc_var_strict_mono)
-      apply (simp add: map_map[THEN sym])
-      apply (metis flist_fimage flist_props(2) vdm_enc_var_strict_mono)
-      apply (rule)
-      apply (simp add: fmap_list_binding_fmap typing comp_def xs_def)
-    done
-qed
 
 end
