theories/parser/utp_alpha_pred_parser.thy
@@ -15,11 +15,11 @@ nonterminal uapred and uaexpr and uzdecls and uzdecl
 syntax
   "_uapred_top_clos" :: "uapred \<Rightarrow> bool" ("(1[_])")
   "_uapred_quote"    :: "uapred \<Rightarrow> 'a WF_ALPHA_PREDICATE" ("(1`_`)")
-  "_uapred_brack"    :: "uapred \<Rightarrow> uapred" ("'(_')")
+  "_uapred_brack"    :: "uapred \<Rightarrow> uapred" ("'(_')" [0] 900)
   "_uapred_true"     :: "'a ALPHABET \<Rightarrow> uapred" ("true\<^bsub>_\<^esub>")
   "_uapred_false"    :: "'a ALPHABET \<Rightarrow> uapred" ("false\<^bsub>_\<^esub>")
   "_uapred_var"      :: "pttrn \<Rightarrow> uapred" ("(_)")
-  "_uapred_evar"     :: "idt \<Rightarrow> uapred" ("$_")
+(*  "_uapred_evar"     :: "idt \<Rightarrow> uapred" ("$_") *)
   "_uapred_and"      :: "uapred \<Rightarrow> uapred \<Rightarrow> uapred" (infixr "\<and>" 35)
   "_uapred_or"       :: "uapred \<Rightarrow> uapred \<Rightarrow> uapred" (infixr "\<or>" 35)
   "_uapred_imp"      :: "uapred \<Rightarrow> uapred \<Rightarrow> uapred" (infixr "\<Rightarrow>" 25)
@@ -31,7 +31,9 @@ syntax
   "_uapred_all1"     :: "pttrn \<Rightarrow> uapred \<Rightarrow> uapred"  ("(3\<forall> _./ _)" [0, 10] 10) 
   "_uapred_exists1"  :: "pttrn \<Rightarrow> uapred \<Rightarrow> uapred"  ("(3\<exists>+ _./ _)" [0, 10] 10) 
   "_uapred_existsres1" :: "pttrn \<Rightarrow> uapred \<Rightarrow> uapred"  ("(3\<exists>- _./ _)" [0, 10] 10) 
+  "_uapred_expr"     :: "uaexpr \<Rightarrow> uapred" ("'(_')" [0] 800)
   "_uapred_equal"    :: "uaexpr \<Rightarrow> uaexpr \<Rightarrow> uapred" (infixl "=" 50)
+  "_uapred_nequal"   :: "uaexpr \<Rightarrow> uaexpr \<Rightarrow> uapred" (infixl "\<noteq>" 50)
   "_uapred_skip"     :: "'a ALPHABET \<Rightarrow> uapred" ("II\<^bsub>_\<^esub>")
   "_uapred_seq"      :: "uapred \<Rightarrow> uapred \<Rightarrow> uapred" (infixr ";" 45)
   "_uapred_cond"     :: "uapred \<Rightarrow> uapred \<Rightarrow> uapred \<Rightarrow> uapred" ("_ \<triangleleft> _ \<triangleright> _")
@@ -52,7 +54,7 @@ translations
   "_uapred_true a"      == "CONST TrueA a"
   "_uapred_false a"     == "CONST FalseA a"
   "_uapred_var x"       => "x"
-  "_uapred_evar x"      == "CONST VarA x"
+(*  "_uapred_evar x"      == "CONST VarA x" *)
   "_uapred_and p q"     == "CONST AndA p q"
   "_uapred_or p q"      == "CONST OrA p q"
   "_uapred_imp p q"     == "CONST ImpliesA p q"
@@ -64,7 +66,9 @@ translations
   "_uapred_all1 x p"    == "CONST ForallA \<lbrace>x\<rbrace> p"
   "_uapred_exists1 x p" == "CONST ExistsA \<lbrace>x\<rbrace> p"
   "_uapred_existsres1 x p" == "CONST ExistsResA \<lbrace>x\<rbrace> p"
+  "_uapred_expr e"      == "CONST ExprA e"
   "_uapred_equal e f"   == "CONST EqualA e f"
+  "_uapred_nequal e f"  == "CONST NotA (CONST EqualA e f)"
   "_uapred_skip"        == "CONST SkipA"
   "_uapred_seq p q"     => "CONST SemiA p q"
   "_uapred_cond p q r"  == "CONST CondA p q r"
@@ -76,23 +80,26 @@ translations
 (* Expression Parser *)
 
 syntax
+  "_uaexpr_brack"    :: "uaexpr \<Rightarrow> uaexpr" ("'(_')" [0] 700)
   "_uaexpr_true"     :: "uaexpr" ("true")
   "_uaexpr_false"    :: "uaexpr" ("false")
   "_uaexpr_var"      :: "pttrn \<Rightarrow> uaexpr" ("_")
-  "_uaexpr_evar"     :: "'a VAR \<Rightarrow> uaexpr" ("$_")
+  "_uaexpr_evar"     :: "'a VAR \<Rightarrow> uaexpr" ("$_" [500] 500)
   "_uaexpr_substp"   :: "uapred \<Rightarrow> uaexpr \<Rightarrow> pttrn \<Rightarrow> uapred" ("(_[_'/_])" [60,60,60] 60)
-  "_uaexpr_member"   :: "uaexpr \<Rightarrow> uaexpr \<Rightarrow> uaexpr" (infix ":" 45)
+   "_uaexpr_member"   :: "uaexpr \<Rightarrow> uaexpr \<Rightarrow> uaexpr" (infix ":" 45)
+  "_uaexpr_coerce"   :: "uaexpr \<Rightarrow> pttrn \<Rightarrow> uaexpr" ("_\<Colon>_" [60,60] 65)
 
 translations
+  "_uaexpr_brack e"      => "e"
   "_uaexpr_true"         == "CONST TrueAE"
   "_uaexpr_false"        == "CONST FalseAE"
   "_uaexpr_var x"        => "x" 
   "_uaexpr_evar x"       == "CONST VarAE x"
   "_uaexpr_substp p e x" == "CONST SubstA p e x"
+  "_uaexpr_coerce e t"   == "CONST CoerceAE e t"
 
-lemma "[[x : A, y : B | $x = false ] \<sqsubseteq> TRUE]"
-  oops
+(* Parser sanity check *)
+term "[[x : A, y : B | $x = false ] \<sqsubseteq> TRUE]"
+term "`$x = ($y) \<and> ($z)`"
 
 end
-
-
